GroupoidModel/Syntax/Injectivity.lean
@@ -18,6 +18,6 @@ axiom EqTp.inv_sigma {Γ A B A' B' l₀ l₁ l₂ l₁' l₂'} :
     (Γ ⊢[l₁] A ≡ A') ∧ ((A, l₁) :: Γ ⊢[l₂] B ≡ B')
 
 /-- Injectivity of Id types. -/
-axiom EqTp.inv_Id {Γ A A' t u t' u' l₀ l l'} :
-    Γ ⊢[l₀] .Id l A t u ≡ .Id l' A' t' u' →
-    l₀ = l ∧ l₀ = l' ∧ (Γ ⊢[l₀] A ≡ A') ∧ (Γ ⊢[l₀] t ≡ t' : A) ∧ (Γ ⊢[l₀] u ≡ u' : A)
+axiom EqTp.inv_Id {Γ A A' t u t' u' l} :
+    Γ ⊢[l] .Id A t u ≡ .Id A' t' u' →
+    (Γ ⊢[l] A ≡ A') ∧ (Γ ⊢[l] t ≡ t' : A) ∧ (Γ ⊢[l] u ≡ u' : A)
