GroupoidModel/Syntax/Synth.lean
@@ -17,11 +17,11 @@ where
   | .pi _ _ A B | .sigma _ _ A B =>
     let l := go Γ A
     max l (go (l :: Γ) B)
-  | .Id _ A _ _ => go Γ A
+  | .Id A _ _ => go Γ A
   | .lam _ _ A b =>
     let l := go Γ A
     max l (go (l :: Γ) b)
-  | .app _ _ B _ a =>
+  | .app _ B _ a =>
     let l := go Γ a
     go (l :: Γ) B
   | .pair _ _ _ t u => max (go Γ t) (go Γ u)
@@ -29,8 +29,8 @@ where
   | .snd _ _ A B _ =>
     let l := go Γ A
     go (l :: Γ) B
-  | .refl _ t => go Γ t
-  | .idRec _ _ _ _ r .. => go Γ r
+  | .refl t => go Γ t
+  | .idRec _ _ _ r .. => go Γ r
   | .univ l => l + 1
   | .el a => go Γ a - 1
   | .code A => go Γ A + 1
@@ -66,12 +66,12 @@ noncomputable def synthTp (Γ : Ctx) : Expr → Expr
   | .bvar 0 => Γ[0]? |>.getD default |>.1.subst Expr.wk
   | .bvar (i+1) => synthTp (Γ.drop 1) (.bvar i) |>.subst Expr.wk
   | .lam l l' A b => .pi l l' A (synthTp ((A, l) :: Γ) b)
-  | .app _ _ B _ a => B.subst a.toSb
+  | .app _ B _ a => B.subst a.toSb
   | .pair l l' B t _ => .sigma l l' (synthTp Γ t) B
   | .fst _ _ A _ _ => A
   | .snd l l' A B p => B.subst (Expr.fst l l' A B p).toSb
-  | .refl l t => .Id l (synthTp Γ t) t t
-  | .idRec _ _ _ M _ u h => M.subst (.snoc u.toSb h)
+  | .refl t => .Id (synthTp Γ t) t t
+  | .idRec _ _ M _ u h => M.subst (.snoc u.toSb h)
   | .code A => .univ (synthLvl Γ A)
   | _ => default
 
